FY/Logic.v
@@ -1,4 +1,4 @@
-From FY Require Import Syntax.
+From FY Require Import Semantics.
 From FY Require Import Map.
 From Coq Require Import Lia.
 
@@ -197,6 +197,8 @@ Proof.
     + apply hoare_asgn.
     + assn_auto'.
 Qed.
+
+
 
 
 
