FY/Semantics.v
@@ -1,0 +1,60 @@
+From FY Require Export Map.
+From FY Require Export Syntax.
+
+Reserved Notation
+         "st '=[' c ']=>' st'"
+         (at level 40, c custom com at level 99,
+          st constr, st' constr at next level).
+Inductive ceval : com -> state -> state -> Prop :=
+  | E_Skip : forall  st,
+      st =[ skip ]=> st
+  | E_Ass : forall  st a n x,
+      aeval st a = n ->
+      st =[ x := a ]=> (x !-> n ; st)
+  | E_Seq : forall  c1 c2 st st' st'',
+      st =[ c1 ]=> st' ->
+      st' =[ c2 ]=> st'' ->
+      st =[ c1 ; c2 ]=> st''
+  | E_IfTrue : forall  st st' b c1 c2,
+      beval st b = true ->
+      st =[ c1 ]=> st' ->
+      st =[ if b then c1 else c2 end]=> st'
+  | E_IfFalse : forall  st st' b c1 c2,
+      beval st b = false ->
+      st =[ c2 ]=> st' ->
+      st =[ if b then c1 else c2 end]=> st'
+  | E_WhileFalse : forall  b st c,
+      beval st b = false ->
+      st =[ while b do c end ]=> st
+  | E_WhileTrue : forall  st st' st'' b c,
+      beval st b = true ->
+      st =[ c ]=> st' ->
+      st' =[ while b do c end ]=> st'' ->
+      st =[ while b do c end ]=> st''
+
+  where "st =[ c ]=> st'" := (ceval c st st').
+
+Definition W : string := "W".
+Definition X : string := "X".
+Definition Y : string := "Y".
+Definition Z : string := "Z".
+
+Example ceval_example1:
+  empty_st =[
+     X := 2;
+     if (X <= 1)
+       then Y := 3
+       else Z := 4
+     end
+  ]=> (Z !-> 4 ; X !-> 2).
+Proof.
+  (* We must supply the intermediate state *)
+  apply E_Seq with (X !-> 2).
+  - (* assignment command *)
+    apply E_Ass. reflexivity.
+  - (* if command *)
+    apply E_IfFalse.
+    reflexivity.
+    apply E_Ass. reflexivity.
+Qed.
+
